---
title: 'ADC and DAC'
date: 2024-07-18
permalink: /posts/2024/07/blog-post-1/
tags:
  - analog-to-digital conversion (ADC)
  - digital-to-analog conversion (DAC)
---

In this blog, we will study analog-to-digital conversion (ADC) and
digital-to-analog conversion (DAC). Down the road, we will prove the well-known
Nyquist sampling theorem. 

The starting point is a continuous-time signal $x(t)$. An ADC takes $x(t)$ and
produces a discrete-time signal $x[n]\triangleq x(nT)$, where $T$ is the
*sampling interval*, also known as *sampling period*. It is also
common to talk about the *sampling rate*, which is defined as $1/T$ if
expressed in Hertz and $2\pi/T$ when expressed in radians per second.

Conversely, a DAC takes a sequence $x[n]$ at its input and produces a
continuous-time waveform $\hat{x}(t)$ at its output. Ideally, if the samples
$x[n]$ preserve all the information in $x(t)$, the DAC will be able to
reconstruct $x(t)$, which theoretically can be expressed as $\hat{x}(t)=x(t)$.

Our first goal is to study under which conditions $x(t)$ can be reconstructed
from $x[n]$.

The notation for Fourier transforms of continuous-time and discrete-time signals
throughout this problem is respectively

$$
\begin{align}
Y(\Omega) \triangleq \int_{-\infty}^{\infty} y(t)e^{-j\Omega t}dt, \quad\quad
    Y(e^{j\omega}) \triangleq \sum_{n=-\infty}^{\infty} y[n]e^{-j\omega n}.
\end{align}
$$

Note the usage of different letters, namely $\Omega$ and $\omega$, in each case.

**1**. The Dirac comb, also known as a train of deltas or train of impulses, is
  $p(t)=\sum_{n=-\infty}^{\infty} \delta(t-Tn)$. The ADC conversion can be
  mathematically thought of as a two-step process. First, $x(t)$ is multiplied
  by a Dirac comb. Let $x_c(t)\triangleq x(t)p(t)$, then we have

  <a id="eq:xc"></a>
  $$
  \begin{align}
    \begin{aligned}
      x_c(t) & = x(t)p(t) = x(t) \sum_{n=-\infty}^{\infty}\delta(t-Tn) \\
          & = \sum_{n=-\infty}^{\infty} x(t)\delta(t-Tn) \overset{(a)}{=} \sum_{n=-\infty}^{\infty} x(nT)\delta(t-Tn) \\
          & = \sum_{n=-\infty}^{\infty} x[n]\delta(t-Tn),
    \end{aligned}
  \end{align}
  $$

  where $(a)$ follows the sampling property, which is
  $x(t)\delta(t-t_0)=x(t_0)\delta(t-t_0)$.

**2**. The second step involves collecting the amplitudes of the resulting deltas to
  extract the sequence $x[n]$. Let us now relate the Fourier transform of
  $x_c(t)$ and that of $x[n]$. 

  $$
  \begin{align}
    \begin{aligned}
      X_c(\omega/T) & =\int_{-\infty}^{\infty} x_c(t)e^{-j(\omega/T) t}dt                                   \\
                  & =\int_{-\infty}^{\infty} \sum_{n=-\infty}^{\infty} x[n]\delta(t-Tn)e^{-j(\omega/T) t}dt \\
                  & =\sum_{n=-\infty}^{\infty} x[n]\int_{-\infty}^{\infty} \delta(t-Tn)e^{-j(\omega/T) t}dt \\
                  & \overset{(a)}{=}\sum_{n=-\infty}^{\infty} x[n]e^{-j\omega n} = X(e^{j\omega}),
    \end{aligned}
  \end{align}
  $$

  where $(a)$ follows the sampling property of the Dirac delta function, which
  is $y(t_0)=\int y(t)\delta(t-t_0)dt$, ($y(t)=e^{-j(\omega/T) t}$ and
  $t_0=Tn$).

**3**. It can be shown that the Fourier transform of $p(t)$ is

  $$
  \begin{align}
    P(\Omega) = \frac{2\pi}{T}\sum_{k=-\infty}^{\infty}\delta\left(\Omega-\frac{2\pi}{T} k\right).
  \end{align}
  $$

  We can find $X_c(\omega/T)$ as following:

  $$
  \begin{align}
    \begin{aligned}
      x_c(t) = x(t)p(t) \overset{\mathcal{F}}{\longrightarrow} X_c(\Omega) & \overset{(a)}{=} \frac{1}{2\pi}X(\Omega)*P(\Omega)           \\
                  & = \frac{1}{2\pi}X(\Omega) * \frac{2\pi}{T}\sum_{k=-\infty}^{\infty}\delta\left(\Omega-\frac{2\pi}{T} k\right)         \\
                  & = \frac{1}{T}\sum_{k=-\infty}^{\infty}X(\Omega) * \delta\left(\Omega-\frac{2\pi}{T} k\right)                          \\
                  & = \frac{1}{T}\sum_{k=-\infty}^{\infty}\int_{-\infty}^{\infty}X(\mu)\delta\left(\Omega-\frac{2\pi}{T} k-\mu\right)d\mu \\
                  & \overset{(b)}{=} \frac{1}{T}\sum_{k=-\infty}^{\infty}X\left(\Omega-\frac{2\pi}{T}k\right),
    \end{aligned}
  \end{align}
  $$

  where $(a)$ follows the property of Fourier transform and $(b)$ follows the
  sampling property of the Dirac delta function.

Observe that the two last parts have established the relation between
the Fourier transform of $x(t)$ and that $x[n]\triangleq x(nT)$: 

<a id="eq:relation"></a>
$$
\begin{align}
  X(e^{j\omega}) = \frac{1}{T}\sum_{k=-\infty}^{\infty}X\left(\frac{\omega-2\pi k}{T}\right).
\end{align}
$$

<!-- 4. As an example to gain insight, suppose that

  $$
  X(\Omega)=\begin{cases}
                0,                                & \text{if }\Omega<-\Omega_0,         \\
                \frac{\Omega_0+\Omega}{\Omega_0}, & \text{if } -\Omega_0\leq\Omega < 0, \\
                \frac{\Omega_0-\Omega}{\Omega_0}, & \text{if } 0\leq\Omega < \Omega_0,  \\
                0,                                & \text{if }\Omega_0\leq\Omega,
            \end{cases}
  $$

  where $\Omega_0$ is a positive constant. Plot $X(\Omega)$, $X_c(\Omega)$, and
  $X(e^{j\omega})$ for the cases where $\Omega_0=(1/3)2\pi/T$ and
  $\Omega_0=(2/3)2\pi/T$. -->

So far, we have established the relation between the Fourier transform
of $x(t)$ and that of $x[n]$. Observe that a continuous-time frequency
$\Omega$ corresponds to a discrete-time frequency $\omega/T$. In other
words:

$$
\begin{align}
  \omega = \Omega T.
\end{align}
$$

We also observed that when the bandwidth of $x(t)$ is greater than half the
sampling rate $(1/2)2\pi/T$, this Fourier transform becomes distorted. Next, we
will proceed to study digital-to-analog conversion.

**4**. The DAC conversion can also be mathematically understood in 2 steps. The
  first is to form $x_c(t)$ from the samples $x[n]$ by using [(2)](#eq:xc). The
  second step involves applying an ideal low-pass filter $g(t)$ with frequency
  response

  $$
  \begin{align}
    G(\Omega)\triangleq\begin{cases}
                            T, & \text{if }|\Omega|<\frac{\pi}{T}, \\
                            0, & \text{otherwise}.
                        \end{cases}
  \end{align}
  $$

  to $x_c(t)$. The continuous-time signal of the above filter is given as

  <a id="eq:filter_in_time"></a>
  $$
  \begin{align}
    g(t) & =\mathcal{F}^{-1}\{G(\Omega)\}=\frac{1}{2\pi}\int_{-\pi/T}^{\pi/T}Te^{j\Omega t}d\Omega =\left[\frac{T}{2\pi}\frac{1}{jt}e^{j\Omega t}\right]_{-\pi/T}^{\pi/T} =\text{sinc}\left(\frac{t}{T}\right).
  \end{align}
  $$

  Therefore,

  $$
  \begin{align}
    \begin{aligned}
      \hat{x}(t) & = x_c(t)*g(t) = \sum_{n=-\infty}^{\infty} x[n]\delta(t-nT)*g(t) = \sum_{n=-\infty}^{\infty} x[n]\delta(t-nT)*\text{sinc}\left(\frac{t}{T}\right) \\
      & = \sum_{n=-\infty}^{\infty} x[n] \int_{-\infty}^{\infty} \text{sinc}\left(\frac{\tau}{T}\right)\delta(t-nT-\tau)d\tau                            \\
      & \overset{(a)}{=} \sum_{n=-\infty}^{\infty} x[n] \text{sinc}\left(\frac{t-nT}{T}\right),
    \end{aligned}
  \end{align}
  $$

  where $(a)$ follows the definition of Dirac delta.

**5**. We say that $x(t)$ is reconstructed from $x[n]$ if $\hat{x}(t)=x(t)$. This is
  the case if $X(\Omega)=0$ for $\Omega\notin (-\pi/T,\pi/T)$, that is, if the
  sampling rate is at least twice the highest frequency (in absolute value) in
  $x(t)$ (Nyquist's sampling theorem). 
  
  Indeed, since $|\Omega-\frac{2\pi}{T}k|\geq|\frac{2\pi}{T}k|-|\Omega|>\pi/T$
  for $k\neq 0$. If $X(\Omega)=0$ for $\Omega\notin (-\pi/T,\pi/T)$, then
  $\sum_{k=-\infty}^{\infty}X\left(\Omega-\frac{2\pi}{T}k\right)=X(\Omega)$. By
  pluging $\omega=\Omega T$ to [(6)](#eq:relation), we have

  <a id="eq:relation2"></a>
  $$
  \begin{align}
      X(e^{j\Omega T}) = \frac{1}{T}\sum_{k=-\infty}^{\infty}X\left(\Omega-\frac{2\pi k}{T}\right) = \frac{1}{T}X(\Omega), \forall \Omega\in (-\pi/T,\pi/T).
  \end{align}
  $$

  Therefore, $X(\Omega)=TX(e^{j\Omega T})$, $\forall \Omega\in (-\pi/T,\pi/T)$.
  
  On the order hand,

  $$
  \begin{align}
    \begin{aligned}
      x(t) & =\mathcal{F}^{-1}\{X(\Omega)\}=T\mathcal{F}^{-1}\{X(e^{j\Omega T})\}=\frac{T}{2\pi}\int_{-\pi/T}^{\pi/T}X(e^{j\Omega T})e^{j\Omega t}d\Omega                                                   \\
      & =\frac{T}{2\pi}\int_{-\pi/T}^{\pi/T}\sum_{n=-\infty}^{\infty}x[n]e^{-j\Omega nT}e^{j\Omega t}d\Omega=\sum_{n=-\infty}^{\infty}x[n]\int_{-\pi/T}^{\pi/T}\frac{T}{2\pi}e^{j\Omega (t-nT)}d\Omega \\
      & =\sum_{n=-\infty}^{\infty}x[n]\left[\frac{T}{2\pi}\frac{1}{j(t-nT)}e^{j\Omega (t-nT)}\right]_{-\pi/T}^{\pi/T}=\sum_{n=-\infty}^{\infty}x[n]\text{sinc}\left(\frac{t-nT}{T}\right)                    \\
      & =\hat{x}(t).
    \end{aligned}
  \end{align}
  $$

<!-- Headings are cool
======

You can have many headings
======

Aren't headings cool?
------ -->